...미친. 그냥 Tr 하나 증명하는 것만 해도 미치게 어렵네;;

Nemonuri/Examples/BeverageVendingMachineRevisited.lean
@@ -43,6 +43,7 @@ def State.eval (s: State) (var: Var) : Val :=
   | .nsoda => s.nsoda |> .mk
   | .nbeer => s.nbeer |> .mk
 
+@[simp]
 instance : ProgramGraph.EvalLike State Var Val where
   coe s := .mk (s.eval)
   coe_injective := by
@@ -74,16 +75,119 @@ inductive Guard where
 
 namespace Guard
 
+open PropositionalLogics
+open ProgramGraph
+
+instance : Inhabited Var := ⟨.nsoda⟩
+
+attribute [local simp] standardType StandardType.isSafe_iff in
+def toFormula (g: Guard) : Formula standardType.AtomicProp :=
+  match g with
+  | .true => .true
+  | .nsoda_gt_zero => .atom ⟨.nsoda, fun val => val.val.val > 0, by simp⟩ ∧ₚ .true
+  | .nbeer_gt_zero => .atom ⟨.nbeer, fun val => val.val.val > 0, by simp⟩ ∧ₚ .true
+  | .nsoda_eq_zero_and_nbeer_eq_zero =>
+    let ap1 : standardType.AtomicProp := ⟨.nsoda, fun val => val.val.val = 0, by simp⟩
+    let ap2 : standardType.AtomicProp := ⟨.nbeer, fun val => val.val.val = 0, by simp⟩
+    (.atom (ap1)) ∧ₚ (.atom (ap2)) ∧ₚ .true
 
 
+theorem toFormula_is_cond (g: Guard) : standardType.IsCond (toFormula g) := by
+  cases g
+  · simp [toFormula]
+  · refine .cons _ _ ?_; simp
+  · refine .cons _ _ ?_; simp
+  · refine .cons _ _ ?_
+    refine .cons _ _ ?_
+    simp
+
+theorem toFormula_injective : Function.Injective toFormula := by
+  intro g1 g2 lm1
+  cases g1 <;> cases g2 <;> simp <;> simp [toFormula] at lm1
+
+
+instance : ProgramGraph.CondLike Guard State Var Val where
+  standardType := standardType
+  toCond g := .mk (g.toFormula) g.toFormula_is_cond
+  toCond_Injective := by
+    intro _ _
+    simp
+    exact toFormula_injective.eq_iff.mp
+
+attribute [local simp] StandardType.isSafe_iff in
+def initial : ProgramGraph.Cond State Var Val standardType where
+  formula := (.atom (⟨.nsoda, fun val => val.val.val = 2, by simp [standardType]⟩)) ∧ₚ .true
+  valid := by
+    refine .cons _ _ ?_
+    simp
 
 end Guard
 
-/-
-instance : ProgramGraph.CondLike Guard State Var Val where
-  standardType := standardType
-  toCond
--/
+def effect (act: Act) (st1: State) : State :=
+  match act with
+  | .coin | .ret_coin => st1
+  | .refill => .mk 2 2
+  | .sget => { st1 with nsoda := st1.nsoda - 1 }
+  | .bget => { st1 with nbeer := st1.nbeer - 1 }
+
+
+inductive Ctr : Loc → Guard → Act → Loc → Prop where
+  | coin : Ctr .start .true .coin .select
+  | refill : Ctr .start .true .refill .start
+  | sget : Ctr .select .nsoda_gt_zero .sget .start
+  | bget : Ctr .select .nbeer_gt_zero .bget .start
+  | ret_coin : Ctr .select .nsoda_eq_zero_and_nbeer_eq_zero .ret_coin .start
+
+
+@[reducible]
+def programGraph : ProgramGraph Guard State Var Val where
+  Loc := Loc
+  Act := Act
+  effect := effect
+  g0 := Guard.initial
+  loc0 := fun l => l = .start
+  ctr := Ctr
+
+@[reducible]
+def transitionSystem : TransitionSystem := programGraph.toTransitionSystem
+
+open PropositionalLogics in
+example : transitionSystem.tr (Loc.start, State.mk 2 2) Act.refill (Loc.start, State.mk 2 2) := by
+  dsimp [transitionSystem]
+  refine .intro _ _ Guard.true _ _ ?_ ?_
+  · dsimp
+    exact .refill
+  · dsimp [ProgramGraph.CondLike.standardType, ProgramGraph.CondLike.toCond,
+           SatRel.IsSat, SatRel.defaultAt, Inhabited.default, SatRel.default, DFunLike.coe,
+           EvalLike.toIndicator, EvalLike.coe]
+    simp only [← Indicator.AreEvalToTrue.eq_true_iff]
+    dsimp [Guard.toFormula]
+    dsimp [Indicator.evalFormulaToBool]
+
+open PropositionalLogics in
+example : transitionSystem.tr (Loc.select, State.mk 1 2) Act.sget (Loc.start, State.mk 0 2) := by
+  dsimp [transitionSystem]
+  rw [ProgramGraph.transition_iff]
+  simp
+  exists Guard.nsoda_gt_zero
+  refine ⟨?_, ?_, ?_⟩
+  · exact .sget
+  · dsimp [ProgramGraph.CondLike.standardType, ProgramGraph.CondLike.toCond,
+           SatRel.IsSat, SatRel.defaultAt, Inhabited.default, SatRel.default, DFunLike.coe,
+           EvalLike.toIndicator, EvalLike.coe]
+    simp only [← Indicator.AreEvalToTrue.eq_true_iff]
+    dsimp [Guard.toFormula]
+    dsimp [Indicator.evalFormulaToBool, Indicator.fn]
+    simp
+    dsimp [ProgramGraph.StandardType.indicateAtomicProp, ProgramGraph.EvalLike.coe, DFunLike.coe]
+    dsimp [State.eval]
+    simp
+  · dsimp [effect]
+
+
+
+
+
 end Examples.BeverageVendingMachines.Revisited
 
 end
